up to subtyping

theories/Extraction/NbE.v
@@ -1,33 +1,33 @@
 From Equations Require Import Equations.
 
-From Mctt Require Import LibTactics.
-From Mctt.Core Require Import Base.
-From Mctt.Core.Semantic Require Export NbE.
-From Mctt.Extraction Require Import Evaluation Readback.
+From McPTS Require Import PtsSignature LibTactics.
+From McPTS.Core Require Import Base.
+From McPTS.Core.Semantic Require Export NbE.
+From McPTS.Extraction Require Import Evaluation Readback.
 Import Domain_Notations.
 
 Generalizable All Variables.
 
-Inductive initial_env_order : ctx -> Prop :=
+Inductive initial_env_order {P : PtsSig} : (ctx P) -> Prop :=
 | ie_nil : initial_env_order nil
 | ie_cons :
   `( initial_env_order Γ ->
-     (forall p, initial_env Γ p ->
-           eval_exp_order A p) ->
-     initial_env_order (A :: Γ)).
+     (forall ρ, initial_env Γ ρ ->
+           eval_exp_order A ρ) ->
+     initial_env_order {{{ Γ, A@s }}}).
 
 #[local]
-Hint Constructors initial_env_order : mctt.
+Hint Constructors initial_env_order : mcpts.
 
-Lemma initial_env_order_sound : forall Γ p,
-    initial_env Γ p ->
+Lemma initial_env_order_sound {P : PtsSig} : forall (Γ : ctx P) ρ,
+    initial_env Γ ρ ->
     initial_env_order Γ.
 Proof with (econstructor; intros; functional_initial_env_rewrite_clear; functional_eval_rewrite_clear; mauto).
   induction 1...
 Qed.
 
 #[local]
-Hint Resolve initial_env_order_sound : mctt.
+Hint Resolve initial_env_order_sound : mcpts.
 
 Section InitialEnvImpl.
 
@@ -42,12 +42,12 @@ Section InitialEnvImpl.
     repeat impl_obl_tac1; try econstructor; mauto.
 
   #[tactic="impl_obl_tac",derive(equations=no,eliminator=no)]
-  Equations initial_env_impl G (H : initial_env_order G) : { p | initial_env G p } by struct H :=
+  Equations initial_env_impl {P : PtsSig} (Γ : ctx P) (H : initial_env_order Γ) : { ρ | initial_env Γ ρ } by struct H :=
   | nil, H => exist _ empty_env _
-  | cons A G, H =>
-      let (p, Hp) := initial_env_impl G _ in
-      let (a, Ha) := eval_exp_impl A p _ in
-      exist _ d{{{ p ↦ ⇑! a (length G) }}} _.
+  | {{{ Γ, A@s }}}, H =>
+      let (ρ, Hρ) := initial_env_impl Γ _ in
+      let (a, Ha) := eval_exp_impl A ρ _ in
+      exist _ d{{{ ρ ↦ ⇑! a (length Γ) }}} _.
 
 End InitialEnvImpl.
 
@@ -56,14 +56,14 @@ End InitialEnvImpl.
     is also obvious from the soundness of eval orders and functional
     nature of initial_env. *)
 
-Lemma initial_env_impl_complete : forall G p,
-    initial_env G p ->
-    exists H H', initial_env_impl G H = exist _ p H'.
+Lemma initial_env_impl_complete {P : PtsSig} : forall (Γ : ctx P) ρ,
+    initial_env Γ ρ ->
+    exists H H', initial_env_impl Γ H = exist _ ρ H'.
 Proof.
   intros.
-  assert (Horder : initial_env_order G) by mauto.
+  assert (Horder : initial_env_order Γ) by mauto.
   exists Horder.
-  destruct (initial_env_impl G Horder).
+  destruct (initial_env_impl Γ Horder).
   functional_initial_env_rewrite_clear.
   eexists; reflexivity.
 Qed.
@@ -86,26 +86,26 @@ Ltac functional_nbe_complete :=
       end
   end.
 
-Inductive nbe_order G M A : Prop :=
+Inductive nbe_order {P : PtsSig} (Γ : ctx P) M A : Prop :=
 | nbe_order_run :
-  `( initial_env_order G ->
-     (forall p, initial_env G p ->
-           eval_exp_order A p) ->
-     (forall p, initial_env G p ->
-           eval_exp_order M p) ->
-     (forall p a m,
-         initial_env G p ->
-         {{ ⟦ A ⟧ p ↘ a }} ->
-         {{ ⟦ M ⟧ p ↘ m }} ->
-         read_nf_order (length G) d{{{ ⇓ a m }}}) ->
-     nbe_order G M A ).
+  `( initial_env_order Γ ->
+     (forall ρ, initial_env Γ ρ ->
+           eval_exp_order A ρ) ->
+     (forall ρ, initial_env Γ ρ ->
+           eval_exp_order M ρ) ->
+     (forall ρ a m,
+         initial_env Γ ρ ->
+         {{ ⟦ A ⟧ ρ ↘ a }} ->
+         {{ ⟦ M ⟧ ρ ↘ m }} ->
+         read_nf_order (length Γ) d{{{ ⇓ a m }}}) ->
+     nbe_order Γ M A ).
 
 #[local]
-Hint Constructors nbe_order : mctt.
+Hint Constructors nbe_order : mcpts.
 
-Lemma nbe_order_sound : forall G M A w,
-    nbe G M A w ->
-    nbe_order G M A.
+Lemma nbe_order_sound {P : PtsSig} : forall (Γ : ctx P) M A w,
+    nbe Γ M A w ->
+    nbe_order Γ M A.
 Proof with (econstructor; intros;
             functional_initial_env_rewrite_clear;
             functional_eval_rewrite_clear;
@@ -115,7 +115,7 @@ Proof with (econstructor; intros;
 Qed.
 
 #[local]
-Hint Resolve nbe_order_sound : mctt.
+Hint Resolve nbe_order_sound : mcpts.
 
 Section NbEDef.
 
@@ -130,40 +130,40 @@ Section NbEDef.
     repeat impl_obl_tac1; try econstructor; mauto.
 
   #[tactic="impl_obl_tac",derive(equations=no,eliminator=no)]
-  Equations nbe_impl G M A (H : nbe_order G M A) : { w | nbe G M A w } by struct H :=
-  | G, M, A, H =>
-      let (p, Hp) := initial_env_impl G _ in
-      let (a, Ha) := eval_exp_impl A p _ in
-      let (m, Hm) := eval_exp_impl M p _ in
-      let (w, Hw) := read_nf_impl (length G) d{{{ ⇓ a m }}} _ in
+  Equations nbe_impl {P : PtsSig} (Γ : ctx P) M A (H : nbe_order Γ M A) : { w | nbe Γ M A w } by struct H :=
+  | Γ, M, A, H =>
+      let (ρ, Hρ) := initial_env_impl Γ _ in
+      let (a, Ha) := eval_exp_impl A ρ _ in
+      let (m, Hm) := eval_exp_impl M ρ _ in
+      let (w, Hw) := read_nf_impl (length Γ) d{{{ ⇓ a m }}} _ in
       exist _ w _.
 
 End NbEDef.
 
-Lemma nbe_impl_complete : forall G M A w,
-    nbe G M A w ->
-    exists H H', nbe_impl G M A H = exist _ w H'.
+Lemma nbe_impl_complete {P : PtsSig} : forall (Γ : ctx P) M A w,
+    nbe Γ M A w ->
+    exists H H', nbe_impl Γ M A H = exist _ w H'.
 Proof.
   intros; functional_nbe_complete.
 Qed.
 
-Inductive nbe_ty_order G A : Prop :=
+Inductive nbe_ty_order {P : PtsSig} (Γ : ctx P) A : Prop :=
 | nbe_ty_order_run :
-  `( initial_env_order G ->
-     (forall p, initial_env G p ->
-           eval_exp_order A p) ->
-     (forall p a,
-         initial_env G p ->
-         {{ ⟦ A ⟧ p ↘ a }} ->
-         read_typ_order (length G) a) ->
-     nbe_ty_order G A ).
+  `( initial_env_order Γ ->
+     (forall ρ, initial_env Γ ρ ->
+           eval_exp_order A ρ) ->
+     (forall ρ a,
+         initial_env Γ ρ ->
+         {{ ⟦ A ⟧ ρ ↘ a }} ->
+         read_typ_order (length Γ) a) ->
+     nbe_ty_order Γ A ).
 
 #[local]
-Hint Constructors nbe_ty_order : mctt.
+Hint Constructors nbe_ty_order : mcpts.
 
-Lemma nbe_ty_order_sound : forall G A w,
-    nbe_ty G A w ->
-    nbe_ty_order G A.
+Lemma nbe_ty_order_sound {P : PtsSig} : forall (Γ : ctx P) A w,
+    nbe_ty Γ A w ->
+    nbe_ty_order Γ A.
 Proof with (econstructor; intros;
             functional_initial_env_rewrite_clear;
             functional_eval_rewrite_clear;
@@ -173,7 +173,7 @@ Proof with (econstructor; intros;
 Qed.
 
 #[local]
-Hint Resolve nbe_ty_order_sound : mctt.
+Hint Resolve nbe_ty_order_sound : mcpts.
 
 Section NbETyDef.
 
@@ -188,18 +188,18 @@ Section NbETyDef.
     repeat impl_obl_tac1; try econstructor; mauto.
 
   #[tactic="impl_obl_tac",derive(equations=no,eliminator=no)]
-  Equations nbe_ty_impl G A (H : nbe_ty_order G A) : { w | nbe_ty G A w } by struct H :=
-  | G, A, H =>
-      let (p, Hp) := initial_env_impl G _ in
-      let (a, Ha) := eval_exp_impl A p _ in
-      let (w, Hw) := read_typ_impl (length G) a _ in
+  Equations nbe_ty_impl {P : PtsSig} (Γ : ctx P) A (H : nbe_ty_order Γ A) : { w | nbe_ty Γ A w } by struct H :=
+  | Γ, A, H =>
+      let (ρ, Hρ) := initial_env_impl Γ _ in
+      let (a, Ha) := eval_exp_impl A ρ _ in
+      let (w, Hw) := read_typ_impl (length Γ) a _ in
       exist _ w _.
 
 End NbETyDef.
 
-Lemma nbe_ty_impl_complete : forall G A w,
-    nbe_ty G A w ->
-    exists H H', nbe_ty_impl G A H = exist _ w H'.
+Lemma nbe_ty_impl_complete {P : PtsSig} : forall (Γ : ctx P) A w,
+    nbe_ty Γ A w ->
+    exists H H', nbe_ty_impl Γ A H = exist _ w H'.
 Proof.
   intros; functional_nbe_complete.
 Qed.
